L14 second half

code/L14/workbook.dfy
@@ -185,3 +185,159 @@ method FirstLoop(n:nat)
   }
   assert i == n;
 }
+
+// Monday stop point
+
+function fib(n:nat): nat
+{
+	if n == 0 then 0
+	else if n == 1 then 1
+	else fib(n-1) + fib(n-2)
+}
+
+method SimplerFib(n:nat) returns (b:nat)
+	ensures b == fib(n)
+{
+	var i := 0;
+	b := 0;
+	var c := 1;
+	while i < n
+		invariant 0 <= i <= n
+		invariant b == fib(i)
+		invariant c == fib(i+1)
+	{
+		b, c := c, b + c;
+		i := i + 1;
+	}
+}
+
+method Decreases()
+{
+  var i := 20;
+  while 0 < i
+    invariant 0 <= i
+    {
+      i := i - 1;
+    }
+}
+
+method Decreases2()
+{
+  var i, n := 0, 20;
+  while i < n
+    invariant 0 <= i <= n
+    decreases n - i
+    {
+      i := i + 1;
+    }
+}
+
+method Decreases3()
+{
+  var i, n := 0, 20;
+  while i != n
+    invariant 0 <= i <= n
+    decreases n - i
+    {
+      i := i + 1;
+    }
+}
+
+function fib2(n:nat): nat
+  decreases n
+{
+  if n == 0 then 0
+  else if n == 1 then 1
+  else fib2(n-1) + fib2(n-2)
+}
+
+method FindPartialContract(a: array<int>, key:int) returns (index:int)
+  // partial contract
+  ensures 0 <= index ==> index < a.Length && a[index] == key
+{
+  // can you write code that satisfies this postcondition?
+  // it can be done with one statement.
+	return -1;
+}
+
+method WithQuantifier()
+{
+  assert forall k :: k < k + 1;
+}
+
+method Find(a: array<int>, key:int) returns (index:int)
+  ensures 0 <= index ==> index < a.Length && a[index] == key
+  ensures index < 0 ==> forall k :: 0 <= k < a.Length ==> a[k] != key
+{
+  index := 0;
+  while index < a.Length
+		invariant 0 <= index <= a.Length
+		invariant forall k :: 0 <= k < index ==> a[k] != key
+	{
+    if a[index] == key {
+      return;
+    }
+    index := index + 1;
+  }
+  index := -1;
+}
+
+method FindMax(a: array<int>) returns (maxIndex:int)
+	requires a.Length >= 1
+	ensures 0 <= maxIndex < a.Length && forall k :: 0 <= k < a.Length ==> a[maxIndex] >= a[k]
+{
+	maxIndex := 0;
+	var i := 0;
+  while i < a.Length
+		invariant maxIndex < a.Length
+		invariant 0 <= maxIndex <= i <= a.Length
+		invariant forall k :: 0 <= k < i ==> a[maxIndex] >= a[k]
+	{
+		if a[i] > a[maxIndex] {
+			maxIndex := i;
+		}
+		i := i + 1;
+	}
+}
+
+predicate sorted(a: array<int>)
+	reads a
+{
+  forall j, k :: 0 <= j < k < a.Length ==> a[j] <= a[k]
+}
+
+predicate sortedAndDistinct(a: array<int>)
+	reads a
+{
+  forall j, k :: 0 <= j < k < a.Length ==> a[j] < a[k]
+}
+
+predicate sortedAndNotNull(a: array?<int>)
+	reads a
+{
+  a != null && forall j, k :: 0 <= j < k < a.Length ==> a[j] < a[k]
+}
+
+method BinarySearch(a: array<int>, value: int) returns (index:int)
+  requires 0 <= a.Length && sorted(a)
+  ensures 0 <= index ==> index < a.Length && a[index] == value
+  ensures index < 0 ==> forall k :: 0 <= k < a.Length ==> a[k] != value
+{
+  var low, high := 0, a.Length;
+  while low < high
+    invariant 0 <= low <= high <= a.Length
+    invariant forall i ::
+      0 <= i < a.Length && !(low <= i < high) ==> a[i] != value
+  {   
+      var mid := (low + high) / 2;
+      if a[mid] < value {
+        low := mid + 1;
+      } else if value < a[mid] {
+        high := mid;
+      } else {
+        return mid;
+      }
+  }
+  return -1;
+}
+
